flyweightLatest.bpl
@@ -1,0 +1,559 @@
+type Ref;
+const null: Ref;
+
+var value: [Ref]int;
+var packedMultipleOf: [Ref] bool;
+var fracMultipleOf: [Ref] real;
+
+var packedMultipleOf21: [Ref] bool;
+var fracMultipleOf21: [Ref] real;
+
+var packedMultipleOf16: [Ref] bool;
+var fracMultipleOf16: [Ref] real;
+
+var packedMultipleOf15: [Ref] bool;
+var fracMultipleOf15: [Ref] real;
+
+var packedMultipleOf14: [Ref] bool;
+var fracMultipleOf14: [Ref] real;
+
+var packedMultipleOf33: [Ref] bool;
+var fracMultipleOf33: [Ref] real;
+
+var packedMultipleOf4: [Ref] bool;
+var fracMultipleOf4: [Ref] real;
+
+
+function modulo(x:int, y:int) returns (int);
+axiom (forall x:int, y:int :: {modulo(x,y)} 
+    ((0 <= x) &&(0 < y) ==> (0 <= modulo(x,y) ) && (modulo(x,y) < y) )
+    &&
+    ((0 <= x) &&(y < 0) ==> (0 <= modulo(x,y) ) && (modulo(x,y) < -y) )
+    &&
+    ((x <= 0) &&(0 < y) ==> (-y <= modulo(x,y) ) && (modulo(x,y) <= 0) )
+    &&
+    ((x <= 0) &&(y < 0) ==> (y <= modulo(x,y) ) && (modulo(x,y) <= 0) )
+   ); 
+
+// TODO maybe need to add a field value that holds a, the one we divide by
+procedure PackMultipleOf(a: int, v:int, this:Ref);
+requires (packedMultipleOf[this]==false) &&
+ 	(value[this] == v) && (modulo(v,a) == 0); 
+
+procedure UnpackMultipleOf(a: int, v:int, this:Ref);
+requires packedMultipleOf[this];
+requires fracMultipleOf[this] > 0.0;
+ensures	(value[this] == v) && (modulo(v,a) == 0); 
+
+procedure PackMultipleOf21(v:int, this:Ref);
+requires (packedMultipleOf21[this]==false) &&
+ 	(value[this] == v) && (modulo(v,21) == 0); 
+
+procedure UnpackMultipleOf21(v:int, this:Ref);
+requires packedMultipleOf21[this];
+requires fracMultipleOf21[this] > 0.0;
+ensures	(value[this] == v) && (modulo(v,21) == 0); 
+
+procedure PackMultipleOf16(v:int, this:Ref);
+requires (packedMultipleOf16[this]==false) &&
+ 	(value[this] == v) && (modulo(v,16) == 0); 
+
+procedure UnpackMultipleOf16(v:int, this:Ref);
+requires packedMultipleOf16[this];
+requires fracMultipleOf16[this] > 0.0;
+ensures	(value[this] == v) && (modulo(v,16) == 0);
+
+procedure PackMultipleOf15(v:int, this:Ref);
+requires (packedMultipleOf15[this]==false) &&
+ 	(value[this] == v) && (modulo(v,15) == 0); 
+
+procedure UnpackMultipleOf15(v:int, this:Ref);
+requires packedMultipleOf15[this];
+requires fracMultipleOf15[this] > 0.0;
+ensures	(value[this] == v) && (modulo(v,15) == 0);
+
+procedure PackMultipleOf14(v:int, this:Ref);
+requires (packedMultipleOf14[this]==false) &&
+ 	(value[this] == v) && (modulo(v,14) == 0); 
+
+procedure UnpackMultipleOf14(v:int, this:Ref);
+requires packedMultipleOf14[this];
+requires fracMultipleOf14[this] > 0.0;
+ensures	(value[this] == v) && (modulo(v,14) == 0);
+
+procedure PackMultipleOf33(v:int, this:Ref);
+requires (packedMultipleOf33[this]==false) &&
+ 	(value[this] == v) && (modulo(v,33) == 0); 
+
+procedure UnpackMultipleOf33(v:int, this:Ref);
+requires packedMultipleOf33[this];
+requires fracMultipleOf33[this] > 0.0;
+ensures	(value[this] == v) && (modulo(v,33) == 0);
+
+procedure PackMultipleOf4(v:int, this:Ref);
+requires (packedMultipleOf4[this]==false) &&
+ 	(value[this] == v) && (modulo(v,4) == 0); 
+
+procedure UnpackMultipleOf4(v:int, this:Ref);
+requires packedMultipleOf4[this];
+requires fracMultipleOf4[this] > 0.0;
+ensures	(value[this] == v) && (modulo(v,4) == 0);
+
+procedure ConstructIntCell(x: int, this: Ref);
+	ensures (value[this] == x);
+
+procedure setValue(x: int, this: Ref) 
+modifies value;
+{
+	value[this] := x;
+}
+
+procedure getValueInt(this: Ref) returns (r:int)
+{
+	r:=value[this];
+}
+
+//-------------------
+
+var collegeNumber :[Ref]int;
+var endowment : [Ref]int;
+
+var packedCollegeNumberField : [Ref]bool;
+var fracCollegeNumberField : [Ref]real;
+
+var packedCollegeFacilitiesMany : [Ref]bool;
+var fracCollegeFacilitiesMany : [Ref]real;
+
+var packedCollegeFacilitiesFew : [Ref]bool;
+var fracCollegeFacilitiesFew : [Ref]real;
+
+var packedCollegeFields : [Ref]bool;
+var fracCollegeFields : [Ref]real;
+
+procedure PackCollegeNumberField(c: int, this:Ref);
+requires (packedCollegeNumberField[this]==false) &&
+ 	(collegeNumber[this] == c); 
+
+procedure UnpackCollegeNumberField(c: int, this:Ref);
+requires packedCollegeNumberField[this];
+requires fracCollegeNumberField[this] > 0.0;
+ensures	(collegeNumber[this] == c);
+
+procedure PackCollegeFields(c: int, this:Ref);
+requires (packedCollegeFields[this]==false) &&
+ 	(collegeNumber[this] == c) && (endowment[this] == c*1000 - 5); 
+
+procedure UnpackCollegeFields(c:int, this:Ref);
+requires packedCollegeFields[this];
+requires fracCollegeFields[this] > 0.0;
+ensures	(collegeNumber[this] == c);
+ensures (endowment[this] == c*1000 - 5);
+
+procedure PackCollegeFacilitiesMany(num:int, c:int, this:Ref);
+requires (packedCollegeFacilitiesMany[this] == false);
+//TODO all Pack procedures need to refer to frac also, 
+// not only to packed.
+requires (collegeNumber[this] == c) && (num >= 10 * c);
+
+procedure UnpackCollegeFacilitiesMany(num:int, c:int, this:Ref);
+requires packedCollegeFacilitiesMany[this];
+requires fracCollegeFacilitiesMany[this] > 0.0;
+//TODO all Unpack procedures need to refer to frac also, 
+// not only to packed.
+ensures (collegeNumber[this] == c) && (num >= 10 * c);
+
+procedure PackCollegeFacilitiesFew(num:int, c:int, this:Ref);
+requires (packedCollegeFacilitiesFew[this] == false);
+requires (collegeNumber[this] == c) && (num <= 4 * c);
+
+procedure UnpackCollegeFacilitiesFew(num:int, c:int, this:Ref);
+requires packedCollegeFacilitiesFew[this];
+requires fracCollegeFacilitiesFew[this] > 0.0;
+ensures (collegeNumber[this] == c) && (num <= 4 * c);
+
+procedure ConstructCollege(number:int, this:Ref) 
+modifies collegeNumber, endowment;
+ensures packedCollegeFields[this] &&
+	(fracCollegeFields[this] == 1.0);
+// TODO need to put in statements about the parameters.
+// ensures this#1.0 CollegeFields()[number, (number*1000)-5]
+{
+	collegeNumber[this] := number;
+	endowment[this] := (number *1000) - 5;
+}
+
+procedure getCollegeNumber(this:Ref) returns (r:int)
+ensures packedCollegeNumberField[this] &&
+	(fracCollegeNumberField[this] == 1.0);
+// TODO add statement about value of parameter 
+// ensures this#1.0 CollegeNumberField()[result]
+{
+	r := collegeNumber[this];
+}
+
+// the method that calculates the extrinsic state
+procedure getNumberFacilities(campusNumber:int, this:Ref) returns (r:Ref)
+requires packedCollegeNumberField[this] && 
+	(fracCollegeNumberField[this] == 1.0);
+//TODO have to say what are the current values of the parameters
+// requires this#1 CollegeNumberField(this.collegeNumber)
+ensures packedMultipleOf[r] &&
+	(fracMultipleOf[r] == 1.0);
+//ensures result#1 MultipleOf(this.collegeNumber)
+{
+	call ConstructIntCell(collegeNumber[this] * campusNumber, r);
+	packedMultipleOf[r] := false;
+	call PackMultipleOf(collegeNumber[this], collegeNumber[this] * campusNumber, r);
+	packedMultipleOf[r] := true;
+	fracMultipleOf[r] := 1.0;
+}
+
+procedure checkFewFacilities(num:int, this:Ref) returns (b:bool)
+requires packedCollegeFacilitiesFew[this] &&
+	(fracCollegeFacilitiesFew[this] == 1.0);
+//requires this#1 collegeFacilitiesFew(num)
+ensures packedCollegeFacilitiesFew[this] &&
+	(fracCollegeFacilitiesFew[this] == 1.0);
+//ensures this#1 collegeFacilitiesFew(num)
+{
+	b := (num <= 4 * collegeNumber[this]);
+}
+
+procedure checkManyFacilities(num:int, this:Ref) returns (b:bool)
+requires packedCollegeFacilitiesMany[this] &&
+	(fracCollegeFacilitiesMany[this] == 1.0);
+//requires this#1 collegeFacilitiesMany(num)
+ensures packedCollegeFacilitiesMany[this] &&
+	(fracCollegeFacilitiesMany[this] == 1.0);
+//ensures this#1 collegeFacilitiesMany(num)
+{
+	b := (num >= 10 * collegeNumber[this]);
+}
+
+//---------------------------
+
+type MapIntCollege = [int] Ref;
+
+// Each ApplicationWebsite will have its own map of college.
+// This field is common with ApplicationWebsite.
+
+var mapOfColleges : [Ref]MapIntCollege; 
+
+var maxSize : [Ref]int;
+
+// the type of packed and frac is different here because 
+// we are dealing with maps and they have an extra index, the key, 
+// that we need in order to get to the value.
+var packedIsEntryNull : [Ref, int]bool;
+var fracIsEntryNull : [Ref, int]real;
+
+//TODO maybe this one has to be like the one above
+var packedKeyValuePair : [Ref]bool;
+var fracKeyValuePair : [Ref]real;
+
+var packedMapOfCollegesField : [Ref]bool;
+var fracMapOfCollegesField : [Ref]real;
+
+procedure PackMapOfCollegesField(m:MapIntCollege, this:Ref);
+requires packedMapOfCollegesField[this] == false;
+requires mapOfColleges[this] == m;
+
+procedure UnpackMapOfCollegesField(m:MapIntCollege, this:Ref);
+requires packedMapOfCollegesField[this];
+requires fracMapOfCollegesField[this] > 0.0;
+ensures mapOfColleges[this] == m;
+
+procedure PackKeyValuePair(m:MapIntCollege, key:int, value:Ref, this:Ref);
+requires packedKeyValuePair[this] == false;
+requires mapOfColleges[this] == m;
+requires  (m[key] == value);
+
+procedure UnpackKeyValuePair(m:MapIntCollege, key:int, value:Ref, this:Ref);
+requires packedKeyValuePair[this];
+requires fracKeyValuePair[this] > 0.0;
+ensures mapOfColleges[this] == m;
+ensures (m[key] == value);
+
+procedure PackIsEntryNull(key1 : int, m:MapIntCollege, this:Ref);
+requires  (packedIsEntryNull[this] == false);
+requires (mapOfColleges[this] == m) && (m[key1] == null);
+
+procedure ConstructMapCollege(m: MapIntCollege, max:int, s:int, this: Ref);
+	ensures (mapOfColleges[this] == m) && (maxSize[this] == max);
+
+procedure makeMapNull(i : int, this:Ref)
+modifies mapOfColleges;
+ensures (forall j:int :: ((j<=i) ==> packedIsEntryNull[this, j]));
+{
+if (i==0) {
+	mapOfColleges[this][i] := null;	
+} else {
+	call makeMapNull(i-1, this);
+}
+}
+
+procedure containsKey(key1: int, this:Ref) returns (b:bool)
+requires packedMapOfCollegesField[this] &&
+	(fracMapOfCollegesField[this] == 1.0);
+//requires this#1.0 MapOfCollegesField()
+//ensures (b == true) && (exists c:College ==> (this#1.0 KeyValuePair(key1, c))	 ||
+//	(b == false) && (this#1.0 KeyValuePair(key1, null)) 
+{
+	b := true;
+	if (mapOfColleges[this][key1] == null) {
+		b := false;	
+	} 
+}
+	
+procedure put(key1 : int, college1: Ref, this:Ref) 
+modifies mapOfColleges;
+requires packedMapOfCollegesField[this] &&
+	(fracMapOfCollegesField[this] == 1.0);
+ensures packedKeyValuePair[this] &&
+	(fracKeyValuePair[this] == 1.0);
+{
+	mapOfColleges[this][key1] := college1;	
+}
+	
+procedure get(key1:int, this:Ref) returns (c:Ref)
+requires packedMapOfCollegesField[this] &&
+	(fracMapOfCollegesField[this] == 1.0);
+ensures packedKeyValuePair[this] &&
+	(fracKeyValuePair[this] == 1.0);
+// TODO make sure fraction values are right
+//requires this#1.0 MapOfCollegesField()
+//ensures this#1.0 KeyValuePair(key1, result)
+{
+	c := mapOfColleges[this][key1];
+}
+	
+procedure lookup(collegeNumber:int, this:Ref) returns (r:Ref)
+modifies mapOfColleges;
+requires packedMapOfCollegesField[this] &&
+	(fracMapOfCollegesField[this] == 1.0);
+ensures packedKeyValuePair[this] &&
+	(fracKeyValuePair[this] == 1.0);
+//ensures this#1.0 KeyValuePair(collegeNumber, result)
+{
+var temp:bool;
+var c:Ref;
+call temp := containsKey(collegeNumber, this);
+if (temp == false) 
+	{
+		call ConstructCollege(collegeNumber, c);
+		packedCollegeFields[c] := false;
+		call PackCollegeFields(collegeNumber, c);
+		packedCollegeFields[c] := true;
+		fracCollegeFields[c] := 1.0;
+
+		call put(collegeNumber, c, this);
+	}
+call r:= get(collegeNumber, this);
+}
+
+//--------------------------
+
+var college : [Ref]Ref;
+var campusNumber : [Ref]int;
+var facilities : [Ref]Ref;
+
+var packedStudentApplicationFields : [Ref]bool;
+var fracStudentApplicationFields : [Ref]real;
+
+var packedStudentAppFacilitiesMany : [Ref]bool;
+var fracStudentAppFacilitiesMany : [Ref]real;
+
+var packedStudentAppFacilitiesFew : [Ref]bool;
+var fracStudentAppFacilitiesFew : [Ref]real;
+
+procedure PackStudentApplicationFields(c:Ref, camp:int, this:Ref);
+requires packedStudentApplicationFields[this] == false;
+requires (college[this] == c) && (campusNumber[this] == camp);
+
+procedure UnpackStudentApplicationFields(c:Ref, camp:int, this:Ref);
+requires packedStudentApplicationFields[this];
+ensures (college[this] == c) && (campusNumber[this] == camp);
+
+procedure PackStudentAppFacilitiesMany(col:Ref, c:int, f:Ref, this:Ref);
+requires packedStudentAppFacilitiesMany[this] == false;
+requires (college[this] == col) && (campusNumber[this] == c) &&
+	(facilities[this] == f) && 
+	packedCollegeFacilitiesMany[col] &&
+	(fracCollegeFacilitiesMany[col] > 0.0);
+//TODO add ensures about params in this object proposition
+
+procedure UnpackStudentAppFacilitiesMany(col:Ref, c:int, this:Ref);
+requires packedStudentAppFacilitiesMany[this];
+requires fracStudentAppFacilitiesMany[this] > 0.0;
+ensures (college[this] == col) && (campusNumber[this] == c) &&
+	packedCollegeFacilitiesMany[col] &&
+	(fracCollegeFacilitiesMany[col] > 0.0);
+
+procedure PackStudentAppFacilitiesFew(col:Ref, c:int, this:Ref);
+requires packedStudentAppFacilitiesFew[this] == false;
+requires (college[this] == col) && (campusNumber[this] == c) &&
+	packedCollegeFacilitiesFew[col] &&
+	(fracCollegeFacilitiesFew[col] > 0.0);
+//TODO add ensures about params in this object proposition
+
+procedure UnpackStudentAppFacilitiesFew(col:Ref, c:int, this:Ref);
+requires packedStudentAppFacilitiesFew[this];
+requires fracStudentAppFacilitiesFew[this] > 0.0;
+ensures (college[this] == col) && (campusNumber[this] == c) &&
+	packedCollegeFacilitiesFew[col] &&
+	(fracCollegeFacilitiesFew[col] > 0.0);
+
+procedure ConstructStudentApplication(col:Ref, campusNum:int, this:Ref) 
+modifies college, facilities, campusNumber;
+ensures packedStudentApplicationFields[this] &&
+	(fracStudentApplicationFields[this] == 1.0);
+{
+    var temp: int;
+		college[this] := col;
+		call temp := getNumberFacilities(campusNum, college[this]);
+    facilities[this] := temp;
+		campusNumber[this] := campusNum;	
+}
+	
+procedure changeApplicationFew(newCampusNumber:int, this:Ref)
+modifies campusNumber, facilities;
+requires packedStudentAppFacilitiesFew[this] &&
+	(fracStudentAppFacilitiesFew[this] == 1.0);
+ensures packedStudentAppFacilitiesFew[this] &&
+	(fracStudentAppFacilitiesFew[this] == 1.0);
+{
+  var temp:int;
+	campusNumber[this] := modulo(newCampusNumber, 4);
+	call temp := getNumberFacilities(campusNumber[this], college[this]);
+  facilities[this] := temp;
+}
+
+procedure changeApplicationMany(newCampusNumber:int, this:Ref)
+modifies campusNumber, facilities;
+requires packedStudentAppFacilitiesMany[this] &&
+	(fracStudentAppFacilitiesMany[this] == 1.0);
+ensures packedStudentAppFacilitiesMany[this] &&
+	(fracStudentAppFacilitiesMany[this] == 1.0);
+{
+  var temp:int;
+	campusNumber[this] := newCampusNumber * 10 + 1;
+	call temp := getNumberFacilities(campusNumber[this], college[this]);
+  facilities[this] := temp;
+}
+
+
+procedure checkFacilitiesFew(this:Ref) returns (b:bool)
+requires packedStudentAppFacilitiesFew[this] &&
+	(fracStudentAppFacilitiesFew[this] == 1.0);
+ensures packedStudentAppFacilitiesFew[this] &&
+	(fracStudentAppFacilitiesFew[this] == 1.0);
+{        
+	var temp:bool;
+	call temp := getValueInt(facilities[this]);
+	b := (temp <= 4 * campusNumber[this]);
+}
+
+procedure checkFacilitiesMany(this:Ref) returns (b:bool)
+requires packedStudentAppFacilitiesMany[this] &&
+	(fracStudentAppFacilitiesMany[this] == 1.0);
+ensures packedStudentAppFacilitiesMany[this] &&
+	(fracStudentAppFacilitiesMany[this] == 1.0);
+{       
+	var temp:bool;
+	call temp := getValueInt(facilities[this]);
+	b := (temp >= 10 * campusNumber[this]);
+}
+
+
+//-------------------------
+
+// Each ApplicationWebsite has its own map of college
+// I use mapOfColleges from mapcollege.bpl
+//var mapOfAvailableColleges : [Ref]MapIntCollege;
+
+var packedApplicationWebsiteField : [Ref]bool;
+var fracApplicationWebsiteField : [Ref]real;
+
+procedure PackApplicationWebsiteField(m: MapIntCollege, this:Ref);
+requires (packedApplicationWebsiteField[this]==false) &&
+ 	(mapOfColleges[this] == m); 
+
+procedure UnpackApplicationWebsiteField(m: MapIntCollege, this:Ref);
+requires packedApplicationWebsiteField[this];
+requires fracApplicationWebsiteField[this] > 0.0;
+ensures	(mapOfColleges[this] == m); 
+
+procedure submitApplicationGetCollege(collegeNumber:int, this:Ref) returns (r: Ref)
+modifies mapOfColleges;
+requires packedApplicationWebsiteField[this] && 
+	(fracApplicationWebsiteField[this] > 0.0);
+ensures ( packedCollegeBuildingsFew[r] && 
+	(fracCollegeBuildingsFew[r] > 0.0) ) ||
+	( packedCollegeBuildingsMany[r] &&
+	(fracCollegeBuildingsMany[r] > 0.0) );
+{
+	var college : Ref;
+	call college := lookup(collegeNumber, mapOfColleges[this]);
+	// might be able to say var r : Ref from the beginning
+	r := college;
+}
+
+procedure main(this:Ref) 
+modifies mapOfColleges;
+{
+	var website : Ref;
+	var college, college2 : Ref;
+	var app1, app2 : Ref;
+	var app3, app4 : Ref;
+	assume (college != college2);
+	assume (app1 != app2);
+	assume (app3 != app4);
+	
+	call ConstructApplicationWebsite(5, website);
+	packedApplicationWebsiteField[website] := false;
+	call PackApplicationWebsiteField(mapOfColleges[website], website);
+	packedApplicationWebsiteField[website] := true;
+	fracApplicationWebsiteField[website] := 1.0;
+
+	call college := submitApplicationGetCollege(2, website);
+
+	call ConstructStudentApplication(college, 3, app1);
+	packedStudentAppFacilitiesFew[app1] := false;
+	call PackStudentAppFacilitiesFew(college, 3, app1);
+	packedStudentAppFacilitiesFew[app1] := true;
+	fracStudentAppFacilitiesFew[app1] := 1.0;
+	fracCollegeFacilitiesFew[college] := fracCollegeFacilitiesFew[college] / 2.0;
+
+	call ConstructStudentApplication(college, 2, app2);
+	packedStudentAppFacilitiesFew[app2] := false;
+	call PackStudentAppFacilitiesFew(college, 2, app2);
+	packedStudentAppFacilitiesFew[app2] := true;
+	fracStudentAppFacilitiesFew[app2] := 1.0;
+	fracCollegeFacilitiesFew[college] := fracCollegeFacilitiesFew[college] / 2.0;
+
+	call checkFewFacilities(app1);
+	call changeApplicationFew(34, app1);
+	call checkFewFacilities(app2);
+
+	// ---- code below this is similar to above
+
+	call college2 := submitApplicationGetCollege(56, website);
+
+	call ConstructStudentApplication(college2, 45, app3);
+	packedStudentAppFacilitiesMany[app3] := false;
+	call PackStudentAppFacilitiesMany(college2, 45, app3);
+	packedStudentAppFacilitiesMany[app3] := true;
+	fracStudentAppFacilitiesMany[app3] := 1.0;
+	fracCollegeFacilitiesMany[college] := fracCollegeFacilitiesMany[college2] / 2.0;
+
+	call ConstructStudentApplication(college2, 97, app4);
+	packedStudentAppFacilitiesMany[app4] := false;
+	call PackStudentAppFacilitiesMany(college2, 97, app4);
+	packedStudentAppFacilitiesMany[app4] := true;
+	fracStudentAppFacilitiesMany[app4] := 1.0;
+	fracCollegeFacilitiesMany[college2] := fracCollegeFacilitiesMany[college2] / 2.0;
+
+	call checkFewFacilities(app3);
+	call changeApplicationFew(78, app3);
+	call checkFewFacilities(app4);
+}
